\documentclass{article}
\usepackage[utf8]{inputenc}
\usepackage{setspace}
\usepackage{tikz}
\usetikzlibrary{positioning}
\usepackage{amsfonts}
\usepackage{amssymb}
\usepackage{amsmath}
\usepackage{amsthm}
\usepackage{systeme}
\usepackage{mathtools}
\usepackage{hyperref}

\begin{document}

\section*{Problem 1}

~

\begin{equation*}
    \begin{split}
        &P(X=k)=(1-p)^{k-1}\cdot p\\
        &P(X=n+k|X>n)=\frac{P(X=n+k\cap X>n)}{P(X>n)}\\
        &P(X=n+k|X>n)=\frac{(1-p)^{n+k-1}\cdot p}{(1-p)^n}\\
        &P(X=n+k|X>n)=(1-p)^{k-1}\cdot p=P(X=k)\\
        \Rightarrow&P(X=n+k|X>n)=P(X=k),\forall n,k\geqslant 1\\
    \end{split}
\end{equation*}

\newpage

~

\section*{Problem 2}

~

\subsection*{Question a}

~

\begin{equation*}
    \begin{split}
        &p_k=P(Heads)p_{k+1}+P(Tails)p_{k-1}\\
        &p_k=\frac{1}{2}p_{k+1}+\frac{1}{2}p_{k-1}\\
    \end{split}
\end{equation*}

~

\subsection*{Question b}

~

\begin{equation*}
    \begin{split}
        b_1=&p_1-p_0\\
        =&\frac{1}{2}p_2+\frac{1}{2}p_0-p_0\\
        =&\frac{1}{2}p_2-\frac{1}{2}p_0\\
        =&\frac{1}{2}p_2-\frac{1}{2}\\
        b_2=&p_2-p_1\\
        =&p_2-(\frac{1}{2}p_2+\frac{1}{2}p_0)\\
        =&\frac{1}{2}p_2-\frac{1}{2}\\
        \Rightarrow&b_1=b_2\\
    \end{split}
\end{equation*}

~

\subsection*{Question c}

~

\begin{equation*}
    \begin{split}
        b_k=&p_k-p_{k-1}\\
        =&p_k-(\frac{1}{2}p_k+\frac{1}{2}p_{k-2})\\
        =&\frac{1}{2}p_k-\frac{1}{2}p_{k-2}\\
        b_{k}=&p_{k-1}-p_{k-2}\\
        =&\frac{1}{2}p_k+\frac{1}{2}p_{k-2}-p_{k-2}\\
        =&\frac{1}{2}p_k-\frac{1}{2}p_{k-2}\\
        \Rightarrow&b_k=b_{k-1}\\
        \Rightarrow&b_k=b_{k-1}=...=b_1\leftarrow\text{By induction}\\
        \Rightarrow&b_k=b_1,\forall k\in (0,N]\\
    \end{split}
\end{equation*}

~

\subsection*{Question d}

~

\begin{equation*}
    \begin{split}
        &b_k=b_1\\
        \Rightarrow&\sum_{i=1}^{k}b_i=k\cdot b_1\\
        &b_k=p_k-p_{k-1}\\
        \Rightarrow&\sum_{i=1}^{k}b_i=\sum_{i=1}^{k}p_k-p_{k-1}=p_k-p_0\\
        \Rightarrow&k\cdot b_1=p_k-p_0\\
        \Rightarrow&p_k=k\cdot b_1+p_0\\
    \end{split}
\end{equation*}

~

\subsection*{Question e}

~

\begin{equation*}
    \begin{split}
        &p_k=k\cdot b_1+p_0\\
        &p_N=N\cdot b_1+p_0=0\\
        \Rightarrow&N=-\frac{p_0}{b_1}=-\frac{1}{b_1}\\
        \Rightarrow&p_k=k\cdot b_1+p_0\\
        \Rightarrow&p_k=-\frac{k}{N}+1\\
    \end{split}
\end{equation*}

\end{document}