\documentclass{article}
\usepackage[utf8]{inputenc}
\usepackage{setspace}
\usepackage{tikz}
\usetikzlibrary{positioning}
\usepackage{amsfonts}
\usepackage{amssymb}
\usepackage{amsmath}
\usepackage{amsthm}
\usepackage{systeme}
\usepackage{mathtools}
\usepackage{hyperref}
\usepackage{gensymb}

\begin{document}
\section*{Question 1}

~

\begin{equation*}
    \begin{split}
        &P(X=Y)\\
        =&\sum_{1\leqslant k<n}P(X=k,Y=n)\\
        =&\sum_{n=1}^{\infty}\sum_{k=1}^{n-1}p(1-p)^{k-1}q(1-q)^{n-1}\\
        =&pq\sum_{n=1}^{\infty}\frac{1-(1-p)^{n-1}}{1-(1-p)}(1-q)^{n-1}\\
        =&q\sum_{n=1}^{\infty}(1-(1-p)^{n-1})(1-q)^{n-1}\\
        =&q\sum_{n=1}^{\infty}(1-q)^{n-1}-q\sum_{n=1}^{\infty}(1-p)^{n-1}(1-q)^{n-1}\\
        =&1-\frac{q}{1-(1-p)(1-q)}\\
        =&1-\frac{q}{p+q-pq}\\
        =&\frac{p-pq}{p+q-pq}
    \end{split}
\end{equation*}

\newpage

\section*{Question 2}

~

\begin{equation*}
    \begin{split}
        &\int_{0}^{1}\int_{y}^{2-y}3(2-x)ydxdy\\
        =&\int_{0}^{1}3y(2-2y)dy\\
        =&1\\
    \end{split}
\end{equation*}

~

\subsection*{Problem a}

~

\begin{equation*}
    \begin{split}
        f_X=&\int_{-\infty}^{\infty}3(2-x)ydy\\
        &0<x\leqslant1\\
        =&\int_{0}^{x}3(2-x)ydy\\
        =&\int_{0}^{x}6y-3xydy\\
        =&-frac{3}{2}x^3+3x^2\\
        &1<x\leqslant2\\
        =&\int_{0}^{2-x}3(2-x)ydy\\
        =&\int_{0}^{2-x}6y-2xydy\\
        =&-\frac{3}{2}(x-2)^3\\
        f_Y=&\int_{-\infty}^{\infty}3(2-x)ydx\\
        =&\int_{y}^{2-y}3(2-x)ydx\\
        =&\int_{y}^{2-y}6y-6xydx\\
        =&6y-6y^2\\
    \end{split}
\end{equation*}

~

\subsection*{Problem b}

~

\begin{equation*}
    \begin{split}
        &E[XY]\\
        =&\int_{0}^{1}\int_{y}^{2-y}xy3(2-x)ydxdy\\
        =&\int_{0}^{1}\int_{y}^{2-y}6xy-3x^2y^2dxdy\\
        =&\int_{0}^{1}2y^5-6y^4+4y^2dy\\
        =&\frac{7}{15}\\
    \end{split}
\end{equation*}

~

\subsection*{Problem c}

~

\begin{equation*}
    \begin{split}
        &P(x+y\leqslant1)\\
        =&\int_{0}^{\frac{1}{2}}\int_{y}^{1-y}xy3(2-x)ydxdy\\
        =&3\int_{0}^{\frac{1}{2}}\frac{3}{2}(1-y)ydy\\
        =&\frac{3}{16}\\
    \end{split}
\end{equation*}
\end{document}